Migrated LangContext (and associated lemmas) to its own file

asign6.v
@@ -1,4 +1,5 @@
 From Coq Require Import ssreflect ssrfun ssrbool.
+Require Import Setoid.
 Require Import FunInd.
 Set Implicit Arguments.
 Require Import Coq.Strings.String.
@@ -13,155 +14,35 @@ Require Import lang.
 Require Import hoas.
 Require Import static_semantics.
 Require Import dynamic_semantics.
+Require Import TypingContexts.
+Open Scope LangContext_scope.
 
-Inductive SubContext : ℾ -> ℾ -> Prop :=
-| SubIntro {Γ1 Γ2} : (forall {s τ}, s ∷ τ ∈ Γ1 -> s ∷ τ ∈ Γ2) -> SubContext Γ1 Γ2
-| SubCons s τ {Γ1 Γ2} : SubContext Γ1 Γ2 -> SubContext (ConsEnv s τ Γ1) (ConsEnv s τ Γ2)
-| SubShadow {Γ1 Γ2} Γ' : SubContext Γ1 Γ2 -> SubContext (ShadowEnv Γ1 Γ') (ShadowEnv Γ2 Γ').
-
-Lemma InterpretSubContext {Γ1 Γ2} : SubContext Γ1 Γ2 -> forall {s τ}, s ∷ τ ∈ Γ1 -> s ∷ τ ∈ Γ2.
-  induction 1 => s0 τ0; first done.
-  all:have: forall τ, ContextLookup s0 Γ1 = Some τ -> ContextLookup s0 Γ2 = Some τ
-        by move => ? /InContextP ?; apply/InContextP.
-  all:by move=> IH /InContextP in1; apply/InContextP; move: in1 => /=; program_equiv.
-Qed.
-
-Lemma SubContextRefl Γ : SubContext Γ Γ. done. Qed.
-
-Lemma SubContextTrans {Γ1 Γ2 Γ3} : SubContext Γ1 Γ2 -> SubContext Γ2 Γ3 -> SubContext Γ1 Γ3.
-  by move => /InterpretSubContext ? /InterpretSubContext.
-Qed.
-
-Lemma SubEquiv {Γ1 Γ2} : EquivContext Γ1 Γ2 <-> (SubContext Γ1 Γ2 /\ SubContext Γ2 Γ1).
-  by move: (@InterpretSubContext) (@InterpretEquivContext Γ1 Γ2).
-Qed.
-
-Notation "a ⊆ b" := (SubContext a b) (at level 1, b at next level).
-
-Lemma SubContextConsRight {Γ1 Γ2} : Γ1 ⊆ Γ2 -> forall x τ, x ∉ Γ1 -> Γ1 ⊆ (ConsEnv x τ Γ2).
-  move=> /InterpretSubContext equiv s τ /InContextPn nin.
-  apply SubIntro => s0 τ0.
-  by case: (string_dec s s0) => [<- /InContextP | neq].
-Qed.
-
-Lemma Weakening {Γ e τ} (typchecks1 : Γ ⊢ e ∷ τ) : forall {Γ'}, Γ ⊆ Γ' -> Γ' ⊢ e ∷ τ.
-  by induction typchecks1 => // Γ'' /InterpretSubContext.
+Lemma Weakening {Γ1 e τ Γ2} (sub: Γ1 ⊆ Γ2) : Γ1 ⊢ e ∷ τ -> Γ2 ⊢ e ∷ τ.
+  by rewrite sub.
 Qed.
 
 Ltac weakening := apply/Weakening/(SubContextConsRight (SubContextRefl _)).
 
 Lemma OtherWeakening {s e} (sNotIn : s ∉f e) : forall {Γ τ} (typechecks1 : Γ ⊢ e ∷ τ) {τ'}, (ConsEnv s τ' Γ) ⊢ e ∷ τ.
-  induction sNotIn; intros Γ τ'' typechecks1 τ'; inv typechecks1; econstructor => //=.
-  - specialize (IHsNotIn (ConsEnv x τarg (ConsEnv f (τarg → τret) Γ)) τret type1 τ').
-    apply/(EquivContextAlsoTypechecks IHsNotIn)/EquivContextP => s0 /=.
-    by program_equiv.
-  - apply/(EquivContextAlsoTypechecks type1)/EquivContextP => s0 /=.
-    by program_equiv.
-  - apply/(EquivContextAlsoTypechecks type1)/EquivContextP => s0 /=.
-    by program_equiv.
+  elim: sNotIn; intros; match goal with H: _ ⊢ _ ∷ _ |- _ => inv H end.
+  all: try done.
+  all: econstructor; first done.
+  - by apply/(EquivContextAlsoTypechecks (H _ _ type1 τ'))/EquivContextP => ? /=; program_equiv.
+  - by apply/(EquivContextAlsoTypechecks type1)/EquivContextP => ? /=; program_equiv.
+  - by apply/(EquivContextAlsoTypechecks type1)/EquivContextP => ? /=; program_equiv.
 Qed.
 
-Reserved Notation "a ≡ b % c" (at level 1, b at next level).
-
-Inductive ContextCongruenceModuloS : ℾ -> ℾ -> string -> Prop :=
-| CongModIntro Γ1 Γ2 s :
-    (forall s', (s=s') \/ (forall τ, s' ∷ τ ∈ Γ1 <-> s' ∷ τ ∈ Γ2)) ->
-    (Γ1 ≡ Γ2 % s)
-| CongModCons {Γ1 Γ2 s s' τ} : Γ1 ≡ Γ2 % s -> (ConsEnv s' τ Γ1) ≡ (ConsEnv s' τ Γ2) % s
-| CongModShad {Γ1 Γ2 Γ' s} : Γ1 ≡ Γ2 % s -> (ShadowEnv Γ1 Γ') ≡ (ShadowEnv Γ2 Γ') % s
-where "a ≡ b % c" := (ContextCongruenceModuloS a b c).
-
-Lemma InEquivToNotInEquiv {s Γ1 Γ2} : (forall τ, s ∷ τ ∈ Γ1 <-> s ∷ τ ∈ Γ2) -> (s ∉ Γ1 <-> s ∉ Γ2).
-  move=> eq1.
-  split => nin1.
-  case (InContextOptions Γ2 s) => //=.
-  move=> [? /eq1/InContextInverse] //=.
-  case (InContextOptions Γ1 s) => //=.
-  move=> [? /eq1/InContextInverse] //=.
-Qed.
-
-Lemma InterpretCongMod' {Γ1 Γ2 s}
-  : Γ1 ≡ Γ2 % s -> forall s', (s=s') \/ (forall τ, s' ∷ τ ∈ Γ1 <-> s' ∷ τ ∈ Γ2).
-  intros H s'.
-  induction H; first done.
-  - decompose [or] IHContextCongruenceModuloS; first done.
-    right; split; inversion 1; done.
-  - decompose [or] IHContextCongruenceModuloS; first done.
-    right; split; inversion 1; done.
-Qed.
-
-Lemma CongModP {Γ1 Γ2 s} :
-  Γ1 ≡ Γ2 % s <-> (forall s0, (string_dec s s0)||(OptionLType_dec (ContextLookup s0 Γ1) (ContextLookup s0 Γ2))).
-  split.
-  - move/InterpretCongMod' => cong s0.
-    apply/orP.
-    case/(_ s0): cong.
-    + left; exact/sumboolP.
-    + right.
-      apply/sumboolP.
-      set o := (ContextLookup _ Γ2).
-      case E : o.
-      * apply/InContextP/b; move/InContextP: E; done.
-      * move/InEquivToNotInEquiv in b.
-        apply/InContextPn/b; move/InContextPn: E; done.
-  - move=> equiv.
-    apply CongModIntro.
-    move=> s0; case/(_ s0)/orP : equiv.
-    + move/sumboolP; done.
-    + move/sumboolP => equiv.
-      right => τ; split => /InContextP eq; exact/InContextP.
-Qed.
-
-Lemma InterpretCongMod {Γ1 Γ2 s}
-  : Γ1 ≡ Γ2 % s -> forall {s'}, s<>s' -> (forall τ, s' ∷ τ ∈ Γ1 <-> s' ∷ τ ∈ Γ2).
-  intros H s' τ H0.
-  edestruct (InterpretCongMod' H s'); done.
-Qed.
-
-Lemma CongModRefl Γ s : Γ ≡ Γ % s.
-  done.
-Qed.
-
-Lemma CongModSymm {Γ1 Γ2 s} : Γ1 ≡ Γ2 % s -> Γ2 ≡ Γ1 % s.
-  by move=> /InterpretCongMod' cong; apply/CongModIntro => s0; move/(_ s0): cong => [|].
-Qed.
-
-Lemma CongModToEquiv {Γ1 Γ2 s} (cong: Γ1 ≡ Γ2 % s) τ : (EquivContext (ConsEnv s τ Γ1) (ConsEnv s τ Γ2)).
-  apply/EquivContextP => s0 /=; case (string_dec s0 s) => //= ne.
-  case/CongModP/(_ s0)/orP: cong => /sumboolP //=.
-Qed.
-
-Lemma CongModConsLeft {x τ Γ1 Γ2} : Γ1 ≡ Γ2 % x -> (ConsEnv x τ Γ1) ≡ Γ2 % x.
-  move => /CongModP cong; apply/CongModP => s0; apply/orP.
-  case/(_ s0)/orP: cong => //= /sumboolP eq.
-  case (string_dec s0 x);[left | right]; exact/sumboolP.
-Qed.
+Hint Resolve (@OtherWeakening).
+Hint Resolve (@Weakening).
 
 Lemma Substitution {e1 Γ1 τ1} (typechks1 : Γ1 ⊢ e1 ∷ τ1) : forall e2 e3 Γ2 τ2 s,
-  (s ∷ τ2 ∈ Γ1) ->
-  Γ2 ⊢ e2 ∷ τ2 ->
-  Γ1 ≡ Γ2 % s ->
-  [e2 / s] e1 = e3 ->
-  Γ2 ⊢ e3 ∷ τ1.
+  (s ∷ τ2 ∈ Γ1) -> Γ2 ⊢ e2 ∷ τ2 -> Γ1 ≡ Γ2 % s -> [e2 / s] e1 = e3 -> Γ2 ⊢ e3 ∷ τ1.
   elim: typechks1; intros; match goal with | H : [ _ / _ ] _ = _ |- _ => inversion H end; subst.
-  - done.
-  - move/InContextP in H; move/InContextP in H0; done.
-  - move/(InterpretCongMod H2 neq) in H; done.
-  - done.
-  - done.
-  - have: s ∷ τ2 ∈ (ConsEnv x τarg (ConsEnv f (τarg → τret) Γ)) by done.
-    have: (ConsEnv x τarg (ConsEnv f (τarg → τret) Γ2)) ⊢ e2 ∷ τ2 by exact/OtherWeakening/OtherWeakening.
-    have: (ConsEnv x τarg (ConsEnv f (τarg → τret) Γ)) ≡ (ConsEnv x τarg (ConsEnv f (τarg → τret) Γ2)) % s
-      by exact/CongModCons/CongModCons.
-    done.
-  - have: f ∷ (τarg → τret) ∈ (ConsEnv x τarg (ConsEnv f (τarg → τret) Γ)) by done.
-    have: (EquivContext (ConsEnv x τarg (ConsEnv f (τarg → τret) Γ)) (ConsEnv x τarg (ConsEnv f (τarg → τret) Γ2)))
-      by exact/EquivCons/CongModToEquiv.
-    by move/EquivContextAlsoTypechecks.
-  - have: x ∷ τarg ∈ (ConsEnv x τarg (ConsEnv f (τarg → τret) Γ)) by done.
-    have: (EquivContext (ConsEnv x τarg (ConsEnv f (τarg → τret) Γ)) (ConsEnv x τarg (ConsEnv f (τarg → τret) Γ2)))
-      by exact/CongModToEquiv/CongModCons.
-    by move/EquivContextAlsoTypechecks.
+  1,4,5,7,8: done.
+  - by move/InContextP in H; move/InContextP in H0.
+  - by move/(InterpretCongMod H2 neq) in H.
+  - by have: s ∷ τ2 ∈ (ConsEnv x τarg (ConsEnv f (τarg → τret) Γ)) /\
+             (ConsEnv x τarg (ConsEnv f (τarg → τret) Γ2)) ⊢ e2 ∷ τ2 by done.
 Qed.
 
 Lemma CannonicalForms {e τ} :
@@ -174,12 +55,7 @@ Lemma CannonicalForms {e τ} :
 Qed.
 
 Lemma TypedEvalContextInversion {Γ E τ0 τ} : Γ ⊢ E {τ0} ∷ τ -> exists x, x ∉ Γ /\ (ConsEnv x τ0 Γ) ⊢ E[x] ∷ τ.
-  destruct 1; simpl.
-  - destruct (ContextFinite Γ) => //=.
-  - by have: (ConsEnv x τ Γ) ⊢ e ∷ ℕ by weakening.
-  - done.
-  - by have: (ConsEnv x τ Γ) ⊢ e ∷ τarg by weakening.
-  - by have: (ConsEnv x τ Γ) ⊢ (AbsExpr fn arg τarg τret body) ∷ (τarg → τret) by weakening.
+  by destruct 1; simpl; first by destruct (ContextFinite Γ).
 Qed.
 
 Lemma DecompositionOfTypes E : forall Γ e0 τ, Γ ⊢ E[e0] ∷ τ -> exists τ1, Γ ⊢ e0 ∷ τ1 /\ Γ ⊢ E {τ1} ∷ τ.
@@ -192,68 +68,58 @@ Lemma DecompositionOfTypes E : forall Γ e0 τ, Γ ⊢ E[e0] ∷ τ -> exists τ
 Qed.
 
 Definition CanStep e := exists e', e ⥛ e'.
+Definition CanStepβ e := exists E e0 e1, e=E[e0] /\ e0 ⥛β e1.
 Definition NotStuck e := 𝕍 e \/ (CanStep e).
+Definition NotStuckβ e := 𝕍 e \/ (CanStepβ e).
 
-Lemma Progressβ : forall {e τ} (ety: NullEnv ⊢ e ∷ τ), (𝕍 e) \/ (exists E e0 e1, e = E[e0] /\ e0 ⥛β e1).
+Hint Constructors EvaluationContext.
+
+Lemma Progressβ : forall {e τ} (ety: NullEnv ⊢ e ∷ τ), NotStuckβ e.
   elim => //=.
   - move=> x τ; inversion 1; inversion H1.
   - move => e1 H1 e2 H2 τ; inversion 1; right.
-    move/(_ NatType type1): H1 => [/(CannonicalForms type1) v1| [E1 [e11 [e12 [-> step1]]]]].
-    all:move/(_ NatType type2): H2 => [/(CannonicalForms type2) v2| [E2 [e21 [e22 [-> step2]]]]].
-    + move: v1 => [n1 ->]; move: v2 => [n2 ->]; exists Hole; exists (AddExpr n1 n2); exists (NatExpr (n1 + n2)); done.
-    + move: v1 => [n1 ->]; exists (EvalContextRAdd n1 E2); exists e21; exists e22; done.
-    + move: v2 => [n2 ->]; exists (EvalContextLAdd E1 n2); exists e11; exists e12; done.
-    + exists (EvalContextLAdd E1 (E2 [e21])); exists e11; exists e12; done.
+    move/(_ NatType type1): H1 => [/(CannonicalForms type1)-[n1 ->]| [E1 [e11 [e12 [-> step1]]]]].
+    all:move/(_ NatType type2): H2 => [/(CannonicalForms type2)-[n2 ->]| [E2 [e21 [e22 [-> step2]]]]].
+    + by exists Hole; exists (AddExpr n1 n2); exists (NatExpr (n1 + n2)).
+    + by exists (EvalContextRAdd n1 E2).
+    + by exists (EvalContextLAdd E1 n2).
+    + by exists (EvalContextLAdd E1 (E2 [e21])).
   - move => e1 H1 e2 H2 τ; inversion 1; right.
-    move/(_ (AbsType τ1 τ) type1): H1 => [/(CannonicalForms type1) v1| [E1 [e11 [e12 [-> step1]]]]].
+    move/(_ (AbsType τ1 τ) type1): H1
+    => [/(CannonicalForms type1)-[f [x [body [nefx ->]]]] | [E1 [e11 [e12 [-> step1]]]]].
     all:move/(_ τ1 type2): H2 => [v2| [E2 [e21 [e22 [-> step2]]]]].
-    + move: v1 => [f [x [body [nefx ->]]]].
-      exists Hole.
-      exists (AppExpr (AbsExpr f x τ1 τ body) e2); simpl.
+    + exists Hole; exists (AppExpr (AbsExpr f x τ1 τ body) e2); simpl.
       move:(@CASAlways e2 x body (AlwaysSafeToSubInto _ _)) => [body' eq].
       move:(@CASAlways (AbsExpr f x τ1 τ body) f body' (AlwaysSafeToSubInto _ _)) => [body'' eq'].
       done.
-    + move: v1 => [f [x [body [nefx ->]]]]; exists (EvalContextRApp f x τ1 τ body E2); exists e21; exists e22; done.
-    + exists (EvalContextLApp E1 e2); exists e11; exists e12; done.
-    + exists (EvalContextLApp E1 (E2 [e21])); exists e11; exists e12; done.
+    + by exists (EvalContextRApp f x τ1 τ body E2).
+    + by exists (EvalContextLApp E1 e2).
+    + by exists (EvalContextLApp E1 (E2 [e21])).
 Qed.
 
 Lemma Progress {e} : forall {τ} (etyp: NullEnv ⊢ e ∷ τ), (NotStuck e).
   by move=> τ /Progressβ; move=> [v | [E [e0 [e1 [-> bstep]]]]].
 Qed.
 
+Hint Resolve Progress.
+
 Lemma βPreservation {e e'} (estep : e ⥛β e') : forall τ (etyp : NullEnv ⊢ e ∷ τ),  NullEnv ⊢ e' ∷ τ.
-  induction estep; intros τ0 etyp; inversion etyp; first done.
-  subst.
-  inversion type1.
-  subst.
-  apply/Substitution.
-  - apply/Substitution.
-    + exact type0.
-    + done.
-    + have: (NullEnv ⊆ (ConsEnv f (τ1 → τ0) NullEnv)) by apply/(SubContextConsRight (SubContextRefl _))/NotInNullEnv.
-      move=> sub; exact/Weakening.
-    + apply/CongModConsLeft/CongModRefl.
-    + done.
-  - apply/InConsEnv.
-  - exact type1.
-  - apply/CongModConsLeft/CongModRefl.
-  - done.
+  induction estep; move=> τ0; inversion 1; first done.
+  subst; inversion type1; subst.
+  (have: ((ConsEnv f (τ1 → τ0) NullEnv) ⊢ e ∷ τ1) by done) => ?.
+  by apply/Substitution; first by apply/Substitution.
 Qed.
 
-Lemma Preservation {e e'} (estep : e ⥛ e') : forall τ (etyp : NullEnv ⊢ e ∷ τ),  NullEnv ⊢ e' ∷ τ.
-  intros τ etyp.
-  inversion estep.
-  subst.
-  move: (DecompositionOfTypes E e1 etyp) => [τn [typee1 ?]].
-  move: (βPreservation betaStep typee1) => etyp1.
+Lemma Preservation {e e'} (estep : e ⥛ e') τ (etyp : NullEnv ⊢ e ∷ τ) : NullEnv ⊢ e' ∷ τ.
+  inversion estep; subst.
+  move: (DecompositionOfTypes E e1 etyp) => [? [/(βPreservation betaStep) ? ?]].
   exact/InterpretTypedEvalContext.
 Qed.
 
+Hint Resolve Preservation.
+
 Lemma Safety {e τ} (etyp : NullEnv ⊢ e ∷ τ) {e'} (estep : e ⥛* e') : (NotStuck e').
-  induction estep.
-  - exact/Progress.
-  - exact/IHestep/Preservation.
+  by induction estep.
 Qed.
 
 
