static_semantics.v
@@ -1,4 +1,5 @@
 From Coq Require Import ssreflect ssrfun ssrbool.
+Require Import Coq.Setoids.Setoid.
 Require Import FunInd.
 Require Import Coq.Strings.String.
 Require Import Coq.Strings.Ascii.
@@ -7,165 +8,9 @@ Require Import Coq.Lists.ListSet.
 Require Import MyBase.
 Require Import lang.
 Require Import hoas.
+Require Import TypingContexts.
 Open Scope MyListScope.
-
-Inductive LangContext : Set :=
-| NullEnv : LangContext
-| ConsEnv (var : string) (typ : 𝕋) (Γ : LangContext) : LangContext
-| ShadowEnv (Γ1 : LangContext) (Γ2 : LangContext) : LangContext.
-Notation ℾ := LangContext.
-
-Bind Scope LangContext_scope with LangContext.
-
-Inductive NotInContext : ℾ -> string -> Prop :=
-| NotInNullEnv {s} : s ∉ NullEnv
-| NotInConsEnv {s1 s2 τ Γ}
-                (diffVars : s1 <> s2)
-                (notInSub : s1 ∉ Γ)
-  : s1 ∉(ConsEnv s2 τ Γ)
-| NotInShadowEnv {s Γ1 Γ2}
-                  (notInLeft : s ∉ Γ1)
-                  (notInRight : s ∉ Γ2)
-  : s ∉ (ShadowEnv Γ1 Γ2)
-where "a ∉ b" := (NotInContext b a) : LangContext_scope.
-
-
-Reserved Notation "a ∷ b ∈ c" (at level 1, no associativity, b at next level).
-Inductive InContext : ℾ -> string -> 𝕋 -> Prop :=
-| InConsEnv {s τ Γ} : s ∷ τ ∈ (ConsEnv s τ Γ)
-| InSubConsEnv {s1 τ1 s2 τ2 Γ}
-               (diffs : s1 <> s2)
-               (inSub : s1 ∷ τ1 ∈ Γ)
-  : s1 ∷ τ1 ∈ (ConsEnv s2 τ2 Γ)
-| InShadowEnvRight {s τ Γ1 Γ2}
-                   (inRight : s ∷ τ ∈ Γ2)
-  : s ∷ τ ∈ (ShadowEnv Γ1 Γ2)
-| InShadowEnvLeft {s τ Γ1 Γ2}
-                  (notInRight : s ∉ Γ2)
-                  (inLeft : s ∷ τ ∈ Γ1)
-  : s ∷ τ ∈ (ShadowEnv Γ1 Γ2)
-where "a ∷ b ∈ c" := (InContext c a b) : LangContext_scope.
 Open Scope LangContext_scope.
-
-Fixpoint ContextLookup s Γ :=
-  match Γ with
-  | NullEnv => None
-  | ConsEnv s0 τ Γ0 =>
-    if (string_dec s s0) then
-      Some τ
-    else ContextLookup s Γ0
-  | ShadowEnv Γ0 Γ1 =>
-    if (ContextLookup s Γ1) is Some τ then
-      Some τ
-    else ContextLookup s Γ0
-  end.
-
-Functional Scheme ContextLookup_ind
-  := Induction for ContextLookup Sort Set.
-
-Lemma InContextPn Γ s : s ∉ Γ <-> (ContextLookup s Γ = None).
-  split.
-  - elim => //=.
-    + move => s1 s2. case (string_dec s1 s2); cbn; done.
-    + move => s0 Γ1 Γ2 notInLeft H notInRight H0; rewrite H; rewrite H0; done.
-  - functional induction (ContextLookup s Γ) => //=.
-    move/IHo => IH; move/(sumboolP (string_dec s s0)): e0; done.
-Qed.
-
-
-Lemma InContextP Γ s τ : s ∷ τ ∈ Γ <-> ContextLookup s Γ = Some τ.
-  split.
-  - elim => //=.
-    + move => s0; case (string_dec s0 s0); cbn; done.
-    + move => s1 τ1 s2; case (string_dec s1 s2); cbn; done.
-    + intros s0 τ0 Γ1 Γ2 inRight H; rewrite H; cbn; done.
-    + move => s0 τ0 Γ1 Γ2 /InContextPn ->; done.
-  - functional induction (ContextLookup s Γ) => //=.
-    + move/(sumboolP (string_dec s s0)): e0 => ->; case => ->; done.
-    + move/IHo => inSub; move/(sumboolP (string_dec s s0)): e0; done.
-    + move/InContextPn : e0 => notInLeft; move/IHo0; done.
-Qed.
-
-Lemma InContextInverse {Γ s τ} : s∷τ ∈ Γ -> s ∉ Γ -> False.
-  move => /InContextP a /InContextPn b; done.
-Qed.
-
-Lemma InContextOptions Γ s : (exists τ, s∷τ∈Γ) \/ (s∉Γ).
-  case E : (ContextLookup s Γ).
-  - move/InContextP: E => //=.
-  - move/InContextPn: E => //=.
-Qed.
-
-Lemma InContextUnique {s τ1 τ2 Γ} : forall (τin1: s ∷ τ1 ∈ Γ) (τin2: s ∷ τ2 ∈ Γ), τ1=τ2.
-  move => /InContextP a /InContextP b; done.
-Qed.
-
-Lemma InConsEnvInversion {s τ τ' Γ} : s ∷ τ ∈ (ConsEnv s τ' Γ) -> τ=τ'.
-  move=> ?; exact: InContextUnique.
-Qed.
-
-Lemma InSubConsEnvInversion {s s' Γ} (neq : s<>s') {τ τ'}
-  : s ∷ τ ∈ (ConsEnv s' τ' Γ) -> s ∷ τ ∈ Γ.
-  inversion 1 => //.
-Qed.
-
-Inductive EquivContext : ℾ -> ℾ -> Prop :=
-| EquivIntro {Γ1 Γ2} : (forall s τ, s ∷ τ ∈ Γ1 <-> s ∷ τ ∈ Γ2) -> EquivContext Γ1 Γ2
-| EquivCons s τ {Γ1 Γ2} : EquivContext Γ1 Γ2 -> EquivContext (ConsEnv s τ Γ1) (ConsEnv s τ Γ2)
-| EquivShadow {Γ1 Γ2} Γ' : EquivContext Γ1 Γ2 -> EquivContext (ShadowEnv Γ1 Γ') (ShadowEnv Γ2 Γ').
-
-Lemma InterpretEquivContext' {Γ1 Γ2} : EquivContext Γ1 Γ2 -> forall {s τ}, s ∷ τ ∈ Γ1 -> s ∷ τ ∈ Γ2.
-Proof with done.
-  elim => //.
-  - move=> s0 τ0 Γ0 Γ3 EquivSub IH s1 τ1; case: (string_dec s1 s0) => [-> | neq] inH.
-    + rewrite (InContextUnique inH (@InConsEnv s0 τ0 Γ0))...
-    + constructor => //; apply IH.
-      pose inSub := InSubConsEnvInversion neq inH...
-  - move=> Γ0 Γ3 Γ' EquivSub IH s τ; inversion 1 => //.
-Qed.
-
-Lemma EquivContextRefl Γ : EquivContext Γ Γ.
-  enough (forall s τ, s ∷ τ ∈ Γ <-> s ∷ τ ∈ Γ); done.
-Qed.
-
-Lemma EquivContextSymm {Γ1 Γ2} : EquivContext Γ1 Γ2 -> EquivContext Γ2 Γ1.
-  elim; done.
-Qed.
-
-Lemma InterpretEquivContext {Γ1 Γ2} : EquivContext Γ1 Γ2 -> (forall {s τ}, s ∷ τ ∈ Γ1 <-> s ∷ τ ∈ Γ2).
-  split.
-  - exact: InterpretEquivContext'.
-  - apply: InterpretEquivContext'; exact: EquivContextSymm.
-Qed.
-
-Lemma EquivContextP Γ1 Γ2 : EquivContext Γ1 Γ2 <-> forall s, ContextLookup s Γ1 = ContextLookup s Γ2.
-  split.
-  - move/InterpretEquivContext => equ s; move/(_ s): equ.
-    case: (InContextOptions Γ1 s) => [[τ i] | /InContextPn ne].
-    + move/(_ τ) => [/(_ i)/InContextP a b]; move/InContextP: i; done.
-    + case: (InContextOptions Γ2 s) => [[τ0 i0] | /InContextPn ne0].
-      * move => eq; move/eq/InContextP : i0 => i0; done.
-      * done.
-  - move=> eq; apply EquivIntro => s τ; split; rewrite 2! InContextP; done.
-Qed.
-
-Lemma EquivContextTrans {Γ1 Γ2 Γ3}
-  : EquivContext Γ1 Γ2 -> EquivContext Γ2 Γ3 -> EquivContext Γ1 Γ3.
-  rewrite 3! EquivContextP; done.
-Qed.
-
-Lemma EquivContextDoubleElim Γ s τ τ'
-  : (EquivContext (ConsEnv s τ (ConsEnv s τ' Γ)) (ConsEnv s τ Γ)).
-  rewrite EquivContextP /= => s0; destruct (string_dec s0 s); cbn; done.
-Qed.
-
-Lemma EquivContextReorder {Γ1 Γ2 s s'} :
-  (EquivContext Γ1 Γ2) -> s<>s' -> forall τ τ',
-      (EquivContext (ConsEnv s τ (ConsEnv s' τ' Γ1)) (ConsEnv s' τ' (ConsEnv s τ Γ2))).
-  rewrite EquivContextP => eq neq τ τ0.
-  rewrite EquivContextP => s0 /=.
-  destruct (string_dec s0 s); destruct (string_dec s0 s') => /=; done.
-Qed.
 
 Reserved Notation "a '⊢' b '∷' c" (at level 1, no associativity, b at next level).
 
@@ -191,9 +36,19 @@ Lemma EquivContextAlsoTypechecks {Γ1 e τ} : Γ1 ⊢ e ∷ τ -> forall {Γ2}, 
   match goal with | [ H: (EquivContext _ _) |- _] => apply/(InterpretEquivContext H) end; done.
 Qed.
 
-Definition OptionLType_dec (s0 s1 : option LType) : {s0=s1} + {s0<>s1}.
-  decide equality.
-  apply LType_dec.
+Hint Resolve (@EquivContextAlsoTypechecks).
+
+Add Parametric Morphism : Typechecks with signature
+    EquivContext ==> eq ==> eq ==> Basics.impl as Typechecks_eq_mor.
+  rewrite /Basics.impl.
+  by move=> *; apply/EquivContextAlsoTypechecks.
+Qed.
+
+Add Parametric Morphism : Typechecks with signature
+    SubContext ++> eq ==> eq ==> Basics.impl as Typechecks_sub_mor.
+  move => Γ1 Γ2 sub e τ.
+  rewrite /Basics.impl; move=> typechecks1; move: Γ2 sub.
+  by induction typechecks1 => // Γ2 /InterpretSubContext.
 Qed.
 
 Fixpoint typchk Γ e :=
@@ -223,39 +78,10 @@ Lemma TypechecksP {Γ e τ} : Γ ⊢ e ∷ τ <-> (typchk Γ e = Some τ).
   - induction 1 => //=; by [apply/InContextP | program_equiv].
   - move: Γ τ; induction e; simpl => Γ τ eq.
     + constructor; exact/InContextP.
-    + by injection eq.
-    + by destruct (OptionLType_dec (typchk Γ e1) (Some NatType));
-        destruct (OptionLType_dec (typchk Γ e2) (Some NatType));
-        try injection eq.
-    + by destruct (string_dec f x);
-        destruct (OptionLType_dec (typchk (ConsEnv x τarg (ConsEnv f (τarg → τret) Γ)) e) (Some τret)); simpl in *;
-          try injection eq.
-    + destruct (typchk Γ e1) eqn:eq1; destruct (typchk Γ e2) eqn:eq2 => //=.
-      all:try destruct l => //=.
-      destruct (LType_dec l1 l0); simpl in * => //=; by injection eq.
-Qed.
-
-Fixpoint ContextVars (Γ : ℾ) :=
-  match Γ with
-  | NullEnv => nil
-  | ConsEnv x τ Γ' => x :: (ContextVars Γ')
-  | ShadowEnv Γ1 Γ2 => ((ContextVars Γ1) ++ (ContextVars Γ2))
-  end.
-
-Functional Scheme ContextVars_ind
-  := Induction for ContextVars Sort Set.
-
-Theorem ContextDomainIsDomain {Γ x} : (~ x ∈ (ContextVars Γ)) <-> x ∉ Γ.
-  split.
-  - functional induction (ContextVars Γ) => //=.
-    + rewrite in_app_iff or_not_iff => [[nin1 nin2]] //=.
-  - induction 1 => //=.
-    + rewrite in_app_iff or_not_iff //=.
-Qed.
-
-Theorem ContextFinite Γ : exists x, x ∉ Γ.
-  destruct (ListFinite (ContextVars Γ)).
-  exists x; move: H; rewrite ContextDomainIsDomain //=.
+    + by case: eq.
+    + move: eq; program_equiv; by [|case].
+    + move: eq; program_equiv; by [|case].
+    + move: eq; program_equiv; by [|case].
 Qed.
 
 Reserved Notation "Γ ⊢ E { τ } ∷ τ'" (at level 1, E at next level, τ at next level, τ' at next level).
