TypingContexts.v
@@ -1,0 +1,265 @@
+From Coq Require Import ssreflect ssrfun ssrbool.
+Require Import Coq.Setoids.Setoid.
+Require Import FunInd.
+Require Import Coq.Strings.String.
+Require Import Coq.Strings.Ascii.
+Require Import Coq.Lists.List.
+Require Import Coq.Lists.ListSet.
+Require Import MyBase.
+Require Import lang.
+Open Scope MyListScope.
+
+Inductive LangContext : Set :=
+| NullEnv : LangContext
+| ConsEnv (var : string) (typ : 𝕋) (Γ : LangContext) : LangContext.
+
+Notation ℾ := LangContext.
+
+Bind Scope LangContext_scope with LangContext.
+
+Inductive NotInContext : ℾ -> string -> Prop :=
+| NotInNullEnv {s} : s ∉ NullEnv
+| NotInConsEnv {s1 s2 τ Γ}
+                (diffVars : s1 <> s2)
+                (notInSub : s1 ∉ Γ)
+  : s1 ∉(ConsEnv s2 τ Γ)
+where "a ∉ b" := (NotInContext b a) : LangContext_scope.
+
+
+Reserved Notation "a ∷ b ∈ c" (at level 1, no associativity, b at next level).
+Inductive InContext : ℾ -> string -> 𝕋 -> Prop :=
+| InConsEnv {s τ Γ} : s ∷ τ ∈ (ConsEnv s τ Γ)
+| InSubConsEnv {s1 τ1 s2 τ2 Γ}
+               (diffs : s1 <> s2)
+               (inSub : s1 ∷ τ1 ∈ Γ)
+  : s1 ∷ τ1 ∈ (ConsEnv s2 τ2 Γ)
+where "a ∷ b ∈ c" := (InContext c a b) : LangContext_scope.
+Open Scope LangContext_scope.
+
+Hint Constructors InContext NotInContext.
+
+Fixpoint ContextLookup s Γ :=
+  match Γ with
+  | NullEnv => None
+  | ConsEnv s0 τ Γ0 =>
+    if (string_dec s s0) then
+      Some τ
+    else ContextLookup s Γ0
+  end.
+
+Functional Scheme ContextLookup_ind
+  := Induction for ContextLookup Sort Set.
+
+Lemma InContextPn Γ s : s ∉ Γ <-> (ContextLookup s Γ = None).
+  split.
+  - by elim => /= *; program_equiv.
+  - by functional induction (ContextLookup s Γ) => //= /IHo IH; move/(sumboolP _): e0.
+Qed.
+
+
+Lemma InContextP Γ s τ : s ∷ τ ∈ Γ <-> ContextLookup s Γ = Some τ.
+  split.
+  - elim => //=; by [move=> *; program_equiv | move=> s0 τ0 Γ1 Γ2 /InContextPn ->].
+  - functional induction (ContextLookup s Γ) => //=.
+    + by move/(sumboolP _): e0 => ->; case.
+    + by move/(sumboolP _): e0 => ? /IHo.
+Qed.
+
+Lemma InContextInverse {Γ s τ} : s∷τ ∈ Γ -> s ∉ Γ -> False.
+  by rewrite InContextP InContextPn.
+Qed.
+
+Lemma InContextOptions Γ s : (exists τ, s∷τ∈Γ) \/ (s∉Γ).
+  case E : (ContextLookup s Γ); by [move/InContextP: E | move/InContextPn: E].
+Qed.
+
+Lemma InContextUnique {s τ1 τ2 Γ} : forall (τin1: s ∷ τ1 ∈ Γ) (τin2: s ∷ τ2 ∈ Γ), τ1=τ2.
+  by rewrite ! InContextP.
+Qed.
+
+Lemma InConsEnvInversion {s τ τ' Γ} (inCons: s ∷ τ ∈ (ConsEnv s τ' Γ)) : τ=τ'.
+  exact: InContextUnique.
+Qed.
+
+Lemma InSubConsEnvInversion {s s' Γ} (neq : s<>s') {τ τ'} : s ∷ τ ∈ (ConsEnv s' τ' Γ) -> s ∷ τ ∈ Γ.
+  by inversion 1.
+Qed.
+
+Inductive EquivContext : ℾ -> ℾ -> Prop :=
+| EquivIntro {Γ1 Γ2} : (forall s τ, s ∷ τ ∈ Γ1 <-> s ∷ τ ∈ Γ2) -> EquivContext Γ1 Γ2
+| EquivCons s τ {Γ1 Γ2} : EquivContext Γ1 Γ2 -> EquivContext (ConsEnv s τ Γ1) (ConsEnv s τ Γ2).
+
+Lemma InterpretEquivContext' {Γ1 Γ2} : EquivContext Γ1 Γ2 -> forall {s τ}, s ∷ τ ∈ Γ1 -> s ∷ τ ∈ Γ2.
+  elim => //.
+  - move=> s0 τ0 Γ0 Γ3 EquivSub IH s1 τ1; case: (string_dec s1 s0) => [-> | neq] inH.
+    + by rewrite (InContextUnique inH InConsEnv).
+    + by move/(InSubConsEnvInversion _) in inH.
+Qed.
+
+Lemma EquivContextRefl Γ : EquivContext Γ Γ. done. Qed.
+
+Lemma EquivContextSymm {Γ1 Γ2} : EquivContext Γ1 Γ2 -> EquivContext Γ2 Γ1. by elim. Qed.
+
+Lemma InterpretEquivContext {Γ1 Γ2} : EquivContext Γ1 Γ2 -> (forall {s τ}, s ∷ τ ∈ Γ1 <-> s ∷ τ ∈ Γ2).
+  by split; apply/InterpretEquivContext';[|apply/EquivContextSymm].
+Qed.
+
+Lemma EquivContextTrans {Γ1 Γ2 Γ3}
+  : EquivContext Γ1 Γ2 -> EquivContext Γ2 Γ3 -> EquivContext Γ1 Γ3.
+  move=> /InterpretEquivContext ? /InterpretEquivContext ?; exact/EquivIntro.
+Qed.
+
+Add Parametric Relation : LangContext EquivContext
+    reflexivity proved by EquivContextRefl
+    symmetry proved by @EquivContextSymm
+    transitivity proved by @EquivContextTrans
+      as EquivContext_rel.
+
+Add Parametric Morphism s : (ContextLookup s) with signature
+    (EquivContext) ==> (eq) as ContextLookup_mor.
+  move=> Γ1 Γ2 /InterpretEquivContext/(_ s).
+  case: (InContextOptions Γ1 s) => [[τ i] | /InContextPn ne].
+  + by move/(_ τ) => [/(_ i)/InContextP a b]; move/InContextP: i.
+  + by case: (InContextOptions Γ2 s) => [[τ0 i0] eq | /InContextPn ne0 //=]; move/eq/InContextP: i0.
+Qed.
+
+Lemma EquivContextP Γ1 Γ2 : EquivContext Γ1 Γ2 <-> forall s, ContextLookup s Γ1 = ContextLookup s Γ2.
+  split.
+  - by move=> eq ?; rewrite eq.
+  - by move=> eq; apply EquivIntro => *; rewrite ! InContextP.
+Qed.
+
+Lemma EquivContextDoubleElim Γ s τ τ'
+  : (EquivContext (ConsEnv s τ (ConsEnv s τ' Γ)) (ConsEnv s τ Γ)).
+  by rewrite EquivContextP /= => ?; program_equiv.
+Qed.
+
+Lemma EquivContextReorder {Γ1 Γ2 s s'} :
+  (EquivContext Γ1 Γ2) -> s<>s' -> forall τ τ',
+      (EquivContext (ConsEnv s τ (ConsEnv s' τ' Γ1)) (ConsEnv s' τ' (ConsEnv s τ Γ2))).
+  by move=> /EquivContextP *; apply/EquivContextP =>* /=; program_equiv.
+Qed.
+
+Fixpoint ContextVars (Γ : ℾ) :=
+  match Γ with
+  | NullEnv => nil
+  | ConsEnv x τ Γ' => x :: (ContextVars Γ')
+  end.
+
+Functional Scheme ContextVars_ind
+  := Induction for ContextVars Sort Set.
+
+Theorem ContextDomainIsDomain {Γ x} : (~ x ∈ (ContextVars Γ)) <-> x ∉ Γ.
+  by split;[functional induction (ContextVars Γ)|induction 1]; rewrite //= in_app_iff or_not_iff.
+Qed.
+
+Theorem ContextFinite Γ : exists x, x ∉ Γ.
+  by move:(ListFinite (ContextVars Γ))=>[x /ContextDomainIsDomain].
+Qed.
+
+Inductive SubContext : ℾ -> ℾ -> Prop :=
+| SubIntro {Γ1 Γ2} : (forall {s τ}, s ∷ τ ∈ Γ1 -> s ∷ τ ∈ Γ2) -> SubContext Γ1 Γ2
+| SubCons s τ {Γ1 Γ2} : SubContext Γ1 Γ2 -> SubContext (ConsEnv s τ Γ1) (ConsEnv s τ Γ2).
+
+Lemma InterpretSubContext {Γ1 Γ2} : SubContext Γ1 Γ2 -> forall {s τ}, s ∷ τ ∈ Γ1 -> s ∷ τ ∈ Γ2.
+  induction 1 => s0 τ0; first done.
+  all:have: forall τ, ContextLookup s0 Γ1 = Some τ -> ContextLookup s0 Γ2 = Some τ
+        by move => ? /InContextP ?; apply/InContextP.
+  all:by move=> IH /InContextP in1; apply/InContextP; move: in1 => /=; program_equiv.
+Qed.
+
+Lemma SubContextRefl Γ : SubContext Γ Γ. done. Qed.
+
+Lemma SubContextTrans {Γ1 Γ2 Γ3} : SubContext Γ1 Γ2 -> SubContext Γ2 Γ3 -> SubContext Γ1 Γ3.
+  by move => /InterpretSubContext ? /InterpretSubContext.
+Qed.
+
+Lemma SubEquiv {Γ1 Γ2} : EquivContext Γ1 Γ2 <-> (SubContext Γ1 Γ2 /\ SubContext Γ2 Γ1).
+  by move: (@InterpretSubContext) (@InterpretEquivContext Γ1 Γ2).
+Qed.
+
+Notation "a ⊆ b" := (SubContext a b) (at level 1, b at next level).
+
+Lemma SubContextConsRight {Γ1 Γ2} : Γ1 ⊆ Γ2 -> forall x τ, x ∉ Γ1 -> Γ1 ⊆ (ConsEnv x τ Γ2).
+  move=> /InterpretSubContext equiv s τ /InContextPn nin.
+  apply SubIntro => s0 τ0.
+  by case: (string_dec s s0) => [<- /InContextP | neq].
+Qed.
+
+Add Parametric Relation : LangContext SubContext
+    reflexivity proved by SubContextRefl
+    transitivity proved by @SubContextTrans
+      as SubContext_rel.
+
+Reserved Notation "a ≡ b % c" (at level 1, b at next level).
+
+Inductive ContextCongruenceModuloS : ℾ -> ℾ -> string -> Prop :=
+| CongModIntro Γ1 Γ2 s :
+    (forall s', (s=s') \/ (forall τ, s' ∷ τ ∈ Γ1 <-> s' ∷ τ ∈ Γ2)) ->
+    (Γ1 ≡ Γ2 % s)
+| CongModCons {Γ1 Γ2 s s' τ} : Γ1 ≡ Γ2 % s -> (ConsEnv s' τ Γ1) ≡ (ConsEnv s' τ Γ2) % s
+where "a ≡ b % c" := (ContextCongruenceModuloS a b c).
+
+Lemma InEquivToNotInEquiv {s Γ1 Γ2} (eq1: forall τ, s ∷ τ ∈ Γ1 <-> s ∷ τ ∈ Γ2) : (s ∉ Γ1 <-> s ∉ Γ2).
+  split => nin1.
+  by case (InContextOptions Γ2 s) => //=; move=> [? /eq1/InContextInverse].
+  by case (InContextOptions Γ1 s) => //=; move=> [? /eq1/InContextInverse].
+Qed.
+
+Lemma InterpretCongMod' {Γ1 Γ2 s}
+  : Γ1 ≡ Γ2 % s -> forall s', (s=s') \/ (forall τ, s' ∷ τ ∈ Γ1 <-> s' ∷ τ ∈ Γ2).
+  intros H s'.
+  induction H; first done.
+  - decompose [or] IHContextCongruenceModuloS; first done.
+    right; split; inversion 1; done.
+Qed.
+
+Lemma CongModP {Γ1 Γ2 s} :
+  Γ1 ≡ Γ2 % s <-> (forall s0, (string_dec s s0)||(OptionLType_dec (ContextLookup s0 Γ1) (ContextLookup s0 Γ2))).
+  split.
+  - move/InterpretCongMod' => cong s0.
+    apply/orP.
+    case/(_ s0): cong.
+    + left; exact/sumboolP.
+    + right.
+      apply/sumboolP.
+      set o := (ContextLookup _ Γ2).
+      case E : o.
+      * apply/InContextP/b; move/InContextP: E; done.
+      * move/InEquivToNotInEquiv in b.
+        apply/InContextPn/b; move/InContextPn: E; done.
+  - move=> equiv.
+    apply CongModIntro.
+    move=> s0; case/(_ s0)/orP : equiv.
+    + move/sumboolP; done.
+    + move/sumboolP => equiv.
+      right => τ; split => /InContextP eq; exact/InContextP.
+Qed.
+
+Lemma InterpretCongMod {Γ1 Γ2 s} (congMod: Γ1 ≡ Γ2 % s) {s'} (neq: s<>s') τ : s' ∷ τ ∈ Γ1 <-> s' ∷ τ ∈ Γ2.
+  by edestruct (InterpretCongMod' congMod s').
+Qed.
+
+Lemma CongModRefl Γ s : Γ ≡ Γ % s. done. Qed.
+
+Lemma CongModSymm {Γ1 Γ2 s} : Γ1 ≡ Γ2 % s -> Γ2 ≡ Γ1 % s.
+  by move=> /InterpretCongMod' cong; apply/CongModIntro => s0; move/(_ s0): cong => [|].
+Qed.
+
+Lemma CongModToEquiv {Γ1 Γ2 s} (cong: Γ1 ≡ Γ2 % s) τ : (EquivContext (ConsEnv s τ Γ1) (ConsEnv s τ Γ2)).
+  apply/EquivContextP => s0 /=; case (string_dec s0 s) => //= ne.
+  case/CongModP/(_ s0)/orP: cong => /sumboolP //=.
+Qed.
+
+Lemma CongModConsLeft {x τ Γ1 Γ2} : Γ1 ≡ Γ2 % x -> (ConsEnv x τ Γ1) ≡ Γ2 % x.
+  move => /CongModP cong; apply/CongModP => s0; apply/orP.
+  case/(_ s0)/orP: cong => //= /sumboolP eq.
+  case (string_dec s0 x);[left | right]; exact/sumboolP.
+Qed.
+
+Hint Constructors EquivContext ContextCongruenceModuloS SubContext.
+Hint Resolve (@SubContextConsRight).
+Hint Resolve (@SubContextRefl).
+Hint Resolve (@CongModToEquiv).
+Hint Resolve (@CongModConsLeft).
+Hint Resolve (@CongModRefl).
